Co-authored-by: Burdmann <Burdmann@users.noreply.github.com>

theories/quicksort.v
@@ -59,6 +59,23 @@ Proof.
 Qed.
 
 
+Definition sublist (lo : nat) (hi : nat) (l : list nat) :=
+    fst (List.fold_right (fun (ele : nat) (acc : ((list nat)*nat)) =>
+            match acc with
+            | (l,index) => if (lo <=? index) && (index <? hi) then
+                    (ele :: l, index-1)
+                else (l, index-1)
+                end) ([],List.length l - 1) l).
+    
+Compute (sublist 2 5 [0;2;5;3;7;9;5;4;4]).
+Example sublist_example1:
+    sublist 2 5 [0;2;5;3;7;9;5;4;4] = [5;3;7].
+Proof.
+    trivial.
+Qed.
+
+
+
 
 (***************************************
             Shuffle code
@@ -139,6 +156,13 @@ Proof.
     reflexivity.
 Qed.
 
+Lemma partition_left_sort :
+forall l pivot lo hi,
+lo < hi -> hi < List.length l -> lo <= pivot -> pivot <= hi -> ((partition_left l pivot lo hi) = lo) \/ (pivot < (partition_left l pivot lo hi)). 
+Proof.
+    intros l pivot lo hi H H1 H2 H3. left. unfold partition_left. unfold partition_left_func. admit.
+Admitted.
+
 Program Fixpoint partition_right (l : list nat) (pivot : nat) (lo : nat) (hi : nat) {measure (hi-lo)} : nat :=
     match hi <=? lo with
         | true => hi
@@ -167,15 +191,13 @@ Program Fixpoint partition (l : list nat) (pivot : nat) (lo : nat) (initial_lo :
         | false => match (j <=? hi) with
             | true => match (lo <=? i) with 
                 | true => partition (swap l i j) pivot (i+1) initial_lo (j-1)
-                | false => (j,[]) (* will never happen *)
+                | false => (j,[0]) (* will never happen *)
                 end
-            | false => (j,[]) (* will never happen *)
+            | false => (j,[1]) (* will never happen *)
             end
         | true => (j, (swap l initial_lo j))
     end end.
 Next Obligation.
-(* symmetry in Heq_anonymous. apply leb_complete_conv in Heq_anonymous. assert (partition_right l pivot lo hi <= hi). apply partition_right_le. assert (partition_left l pivot lo hi >= lo). apply partition_left_ge.
-apply helper. trivial. trivial. trivial. *)
 symmetry in Heq_anonymous1. apply leb_complete_conv in Heq_anonymous1. symmetry in Heq_anonymous.
 apply Nat.leb_le in Heq_anonymous. symmetry in Heq_anonymous2. apply Nat.leb_le in Heq_anonymous2. apply helper. trivial. trivial. trivial.
 Qed.
@@ -187,7 +209,7 @@ Program Fixpoint sort (l : list nat) (lo : nat) (hi : nat) {measure (hi-lo)} : l
     | true => l
     | false => match (partition l (lookup l lo) lo lo hi) with
         | (j, partitioned) => match ((j <=? hi) && (lo <=? j)) with 
-            | false => l (* will never happen *)
+            | false => [2] (* will never happen *)
             | true => sort (sort partitioned lo (j-1)) (j+1) hi
             end
     end end.
@@ -204,16 +226,6 @@ apply Nat.leb_le in H0.
 lia.
 Qed.
 
-Program Fixpoint sort2 (l : list nat) (lo : nat) (hi : nat) (_:lo<=hi) {measure (hi-lo)} : list nat :=
-    match (hi <=? lo) with
-    | true => l
-    | false => match (partition l (lookup l lo) lo lo hi) with
-        | (j, partitioned) => match ((j <=? hi) && (lo <=? j)) with 
-            | false => l (* will never happen *)
-            | true => sort (sort partitioned lo (j-1)) (j+1) hi
-            end
-    end end.
-
 Definition quicksort (l : list nat) : list nat :=
     match (shuffle l) with
     (* | shuffeled => shuffeled  *)
@@ -222,7 +234,6 @@ Definition quicksort (l : list nat) : list nat :=
 
 Compute (quicksort [15;14;13;12;11;10;5;2;6;3;1;4;9;8;7]).
 Compute (quicksort [66; 91; 69; 62; 52; 10; 49; 38; 53; 54; 98; 95; 92; 6; 20; 32; 41; 71; 59; 25; 80; 75; 73; 79; 63; 48; 12; 46; 28; 68; 65; 24; 81; 85; 47; 35; 33; 30; 17; 72; 7; 89; 40; 39; 94; 51; 13; 11; 67; 16; 76; 31; 77; 60; 82; 61; 42; 18; 36; 87; 93; 88; 26; 22; 8; 4; 84; 29; 21; 97; 56; 2; 37; 90; 9; 15; 50; 58; 70; 78; 19; 99; 86; 44; 96; 1; 100; 14; 43; 64; 55; 3; 27; 45; 74; 0; 23; 57; 34; 5; 83]).
-(* Compute (quicksort [163; 924; 313; 374; 81; 679; 398; 785; 842; 408; 191; 60; 794; 216; 791; 749; 424; 661; 383; 898; 203; 405; 479; 620; 322; 451; 634; 72; 884; 20; 750; 925; 496; 542; 440; 284; 411; 698; 556; 154; 446; 674; 397; 716; 540; 441; 230; 551; 367; 183; 115; 643; 905; 178; 356; 660; 37; 636; 433; 387; 30; 63; 912; 276; 967; 965; 179; 910; 861; 426; 558; 66; 439; 263; 756; 489; 848; 903; 492; 992; 641; 597; 516; 310; 784; 456; 635; 327; 198; 854; 93; 278; 545; 6; 865; 533; 793; 318; 217; 614; 527; 249; 826; 880; 930; 735; 822; 612; 937; 258; 369; 24; 246; 658; 262; 891; 469; 510; 528; 195; 240; 990; 963; 388; 131; 882; 897; 53; 602; 889; 581; 772; 182; 59; 710; 427; 337; 366; 700; 351; 590; 873; 714; 82; 259; 639; 790; 22; 87; 52; 128; 202; 472; 977; 526; 270; 974; 904; 952; 333; 393; 942; 301; 729; 232; 565; 821; 675; 814; 940; 566; 838; 626; 563; 119; 702; 836; 438; 375; 519; 175; 778; 863; 35; 483; 521; 169; 697; 89; 399; 713; 999; 292; 423; 135; 642; 325; 382; 689; 224; 820; 680; 773; 458; 693; 461; 909; 613; 707; 272; 332; 338; 190; 657; 67; 293; 319; 960; 363; 831; 746; 801; 430; 271; 671; 158; 107; 464; 871; 979; 275; 127; 633; 616; 166; 984; 357; 417; 637; 650; 605; 941; 390; 104; 630; 391; 58; 122; 656; 985; 741; 568; 732; 260; 47; 969; 274; 269; 806; 864; 346; 171; 734; 421; 887; 347; 872; 678; 947; 100; 414; 499; 587; 447; 893; 416; 400; 384; 315; 829; 134; 381; 792; 890; 517; 490; 804; 847; 694; 686; 164; 449; 353; 913; 592; 55; 437; 757; 525; 788; 473; 603; 585; 95; 908; 948; 879; 782; 43; 976; 761; 205; 45; 121; 304; 255; 307; 481; 90; 582; 894; 453; 54; 500; 564; 345; 966; 401; 389; 34; 759; 724; 403; 751; 139; 50; 125; 931; 813; 736; 250; 508; 101; 611; 40; 218; 0; 340; 860; 409; 176; 599; 550; 277; 874; 254; 972; 619; 415; 537; 1; 684; 627; 144; 291; 442; 429; 522; 964; 797; 33; 225; 237; 448; 222; 951; 640; 359; 482; 8; 404; 392; 161; 719; 126; 209; 159; 877; 770; 557; 5; 49; 807; 955; 311; 850; 286; 596; 598; 186; 738; 799; 302; 844; 845; 800; 962; 852; 42; 601; 774; 594; 561; 544; 248; 803; 26; 257; 410; 470; 444; 380; 206; 112; 12; 339; 288; 975; 923; 364; 308; 497; 78; 71; 888; 494; 91; 204; 187; 267; 362; 926; 110; 3; 253; 840; 827; 130; 76; 744; 978; 487; 753; 685; 562; 192; 454; 932; 287; 628; 745; 303; 94; 712; 419; 652; 769; 378; 688; 120; 896; 450; 385; 938; 68; 109; 97; 867; 491; 858; 343; 928; 137; 535; 754; 504; 870; 810; 731; 560; 953; 939; 221; 553; 355; 728; 280; 79; 148; 23; 266; 866; 412; 593; 506; 48; 486; 715; 242; 235; 644; 312; 170; 869; 11; 503; 201; 523; 841; 816; 478; 342; 541; 907; 809; 708; 659; 775; 452; 915; 70; 629; 811; 65; 349; 372; 580; 62; 514; 878; 428; 569; 954; 25; 329; 690; 995; 354; 615; 309; 281; 959; 664; 748; 717; 997; 763; 767; 279; 958; 181; 406; 305; 740; 682; 762; 677; 911; 379; 243; 157; 624; 98; 189; 968; 971; 376; 579; 875; 306; 80; 160; 956; 648; 546; 548; 457; 950; 994; 723; 933; 771; 256; 849; 2; 57; 588; 881; 536; 733; 85; 837; 141; 808; 973; 666; 672; 998; 435; 921; 518; 229; 760; 207; 488; 777; 214; 103; 386; 434; 991; 725; 226; 764; 467; 402; 589; 862; 670; 117; 502; 335; 418; 145; 118; 818; 324; 577; 779; 236; 855; 283; 41; 920; 649; 895; 162; 511; 326; 625; 567; 621; 51; 505; 591; 9; 781; 106; 228; 252; 739; 239; 373; 632; 783; 654; 886; 321; 681; 73; 463; 696; 431; 857; 348; 663; 916; 213; 476; 946; 987; 297; 289; 299; 394; 151; 983; 687; 241; 509; 631; 282; 531; 856; 507; 173; 574; 196; 970; 554; 529; 147; 833; 140; 555; 828; 317; 74; 600; 919; 815; 92; 296; 669; 945; 233; 776; 922; 532; 31; 123; 432; 722; 84; 330; 993; 691; 798; 901; 165; 655; 193; 683; 231; 934; 264; 695; 651; 780; 552; 495; 943; 344; 906; 726; 543; 36; 727; 986; 843; 576; 718; 268; 210; 114; 835; 136; 573; 223; 455; 413; 957; 44; 586; 7; 61; 787; 19; 876; 200; 706; 96; 167; 102; 480; 766; 802; 138; 377; 133; 132; 320; 17; 445; 177; 371; 295; 16; 665; 667; 743; 352; 575; 350; 184; 980; 851; 28; 168; 617; 936; 512; 38; 834; 720; 825; 99; 111; 46; 647; 883; 420; 358; 524; 609; 116; 244; 900; 832; 595; 294; 234; 645; 174; 653; 699; 703; 853; 513; 323; 436; 668; 247; 468; 108; 578; 21; 988; 755; 570; 823; 752; 300; 290; 466; 64; 285; 341; 86; 227; 152; 742; 331; 215; 425; 142; 18; 129; 13; 29; 982; 944; 314; 251; 758; 56; 711; 395; 618; 14; 334; 819; 549; 39; 485; 949; 673; 113; 361; 32; 75; 459; 622; 462; 817; 149; 824; 830; 180; 530; 298; 515; 493; 676; 606; 892; 701; 839; 868; 4; 188; 199; 927; 328; 238; 150; 796; 273; 539; 460; 899; 805; 704; 501; 245; 859; 15; 172; 610; 407; 747; 989; 584; 981; 27; 422; 885; 812; 261; 156; 646; 559; 608; 197; 475; 692; 918; 105; 365; 88; 484; 185; 996; 623; 571; 370; 474; 360; 730; 538; 961; 194; 77; 662; 124; 572; 902; 789; 583; 69; 471; 10; 768; 607; 737; 153; 396; 265; 846; 211; 534; 336; 914; 604; 638; 465; 917; 547; 443; 709; 143; 795; 83; 498; 208; 765; 929; 316; 477; 220; 219; 146; 520; 786; 155; 935; 368; 721; 212; 705]). *)
 Example quicksort_example1:
     quicksort [2;3;1;4] = [1;2;3;4].
 Proof.
@@ -273,6 +284,21 @@ Definition sorted'' (al : list nat) := forall i j,
 (** * Proof of Correctness *)
 
 
+Definition sublist_sorted (lo : nat) (hi : nat) (l : list nat) : Prop :=
+lo < hi -> 
+hi < (List.length l) ->
+sorted (sublist lo hi l).
+
+Inductive indexSorted : list nat -> nat -> nat -> Prop :=
+| indSorted_sorted : forall l lo hi,
+    sorted l -> indexSorted l lo hi
+| indSorted_trivial : forall l lo hi,
+    hi < lo -> indexSorted l lo hi
+| indSorted_sort : forall l lo hi,
+    sublist_sorted lo hi l -> indexSorted l lo hi.
+
+Hint Constructors indexSorted.
+
 (*First proof that if l is shuffle it still contains all
  the same elemetns just in a different order*)
 Search (Permutation _ _).
@@ -285,15 +311,22 @@ Proof.
     admit.
 Admitted.
 
-
+Lemma Sort_btw_index :
+    forall l lo hi, 
+   indexSorted (sort l lo hi) lo hi.
+Proof.
+    intros l lo hi. destruct (lo <? hi).
+    - unfold sort. unfold sort_func. apply indSorted_sort. unfold sublist_sorted. intros. destruct l.
+    
+    
 Search(length _).
 Lemma quicksort_sortes:
-    forall l , sorted l -> sorted (quicksort l).
+    forall l , sorted (quicksort l).
 Proof.
-    intros l S. induction l. simpl.
+    intros l. induction l. simpl.
 - trivial.
 - unfold quicksort. induction (shuffle (a :: l)).
     * trivial.
-    * simpl. unfold sort. unfold sort_func.
+    * simpl. unfold sort. unfold sort_func. 
 
     
